Tibi/Typing.lean
@@ -1,21 +1,26 @@
 import Tibi.Basic
+import Tibi.FinInt
 import Tibi.Syntax
 import Tibi.Util
 
 namespace Tibi
 
 inductive Typ
-| Int
+| Int64
 deriving DecidableEq
 
 def Typ.toString : Typ → String
-| .Int => "Int"
+| Int64 => "Int"
 
 instance : ToString Typ where
   toString := Typ.toString
 
 inductive HasType : Expr → Typ → Prop
-| Int {n : Int64} : HasType (.Const n) .Int
+| Int64 {n : Int} (hLt : n < Int64.size) (hGe : n ≥ -Int64.size) : HasType (.Const n) .Int64
 
 def Expr.typeCheck : (e : Expr) → {{ t | HasType e t }}
-| .Const _ => .found .Int .Int
+| .Const n =>
+    if h : (-Int64.size : Int) ≤ n ∧ n < Int64.size then
+      .found .Int64 <| .Int64 h.right h.left
+    else
+      .unknown
