Tibi/Compiler.lean
@@ -6,5 +6,18 @@ namespace Tibi
 
 open Wasm.Value
 
-def Expr.compile : Expr → List Wasm.Instr
-| .Const n => [.i64__const n]
+inductive CompileError
+| OutOfBounds_Int64 (n : Int)
+
+def Expr.compile : Expr → Except CompileError (List Wasm.Instr)
+| .Const n =>
+    if h : (-Int64.size : Int) ≤ n ∧ n < Int64.size then
+      .ok [.i64__const <| Int64.mk ⟨n, h.right, h.left⟩]
+    else
+      .error <| .OutOfBounds_Int64 n
+
+def CompileError.toString : CompileError → String
+| .OutOfBounds_Int64 n => s!"{n} is out of Int64 bounds, should be satisfied that -2{Nat.toSuperscriptString 63} ≤ n < 2{Nat.toSuperscriptString 63}"
+
+instance : ToString CompileError where
+  toString := CompileError.toString
