Tibi/Interpreter.lean
@@ -1,13 +1,13 @@
 import Tibi.Basic
 import Tibi.FinInt
 import Tibi.Syntax
+import Tibi.Semantics
 
 namespace Tibi
 
-inductive EvalError
-
-instance : ToString EvalError where
-  toString _ := "something went wrong"
-
 def Expr.eval : Expr → Except EvalError Int64
-| .Const n => .ok n
+| .Const n =>
+    if h : (-Int64.size : Int) ≤ n ∧ n < Int64.size then
+      .ok <| Int64.mk ⟨n, h.right, h.left⟩
+    else
+      .error <| .OutOfBounds_Int64 n
