Tibi/Props.lean
@@ -1,2 +1,3 @@
 import Tibi.Props.Compiler
+import Tibi.Props.Interpreter
 import Tibi.Props.Typing
