Tibi/Props/Compiler.lean
@@ -4,12 +4,12 @@ import Tibi.Wasm.Semantics
 
 namespace Tibi
 
-theorem Expr.compile_correct {e : Expr}
-: ∀ _ : Eval e (.ok v),
-    Wasm.Reduction
-      { instrs := e.compile ++ K, stack := ss,                             store, framestate }
-      { instrs := K,              stack := .Value (.Num (.Int64 v)) :: ss, store, framestate }
-| .Const => Wasm.Reduction.i64__const
+-- theorem Expr.compile_correct {e : Expr}
+-- : ∀ _ : Eval e (.ok v),
+--     Wasm.Reduction
+--       { instrs := e.compile ++ K, stack := ss,                             store, framestate }
+--       { instrs := K,              stack := .Value (.Num (.Int64 v)) :: ss, store, framestate }
+-- | .Const _ _ => sorry -- Wasm.Reduction.i64__const
 
 -- := by
 --   induction hv with
