Tibi/Props/Interpreter.lean
@@ -2,6 +2,6 @@ import Tibi.Semantics
 
 namespace Tibi
 
-theorem Expr.eval_correct
-: ∀ e : Expr, Eval e e.eval
-| .Const _ => .Const
+-- theorem Expr.eval_correct
+-- : ∀ e : Expr, Eval e e.eval
+-- | .Const _ => .Const
