Tibi/Semantics.lean
@@ -1,8 +1,17 @@
 import Tibi.Basic
 import Tibi.FinInt
-import Tibi.Interpreter
+import Tibi.Syntax
 
 namespace Tibi
 
+inductive EvalError
+| OutOfBounds_Int64 (n : Int)
+
 inductive Eval : Expr → Except EvalError Int64 → Prop
-| Const {n : Int64} : Eval (.Const n) (.ok n)
+| Const {n : Int} (hLe : n < Int64.size) (hGe : n >= -Int64.size) : Eval (.Const n) (.ok <| Int64.mk ⟨n, hLe, hGe⟩)
+
+def EvalError.toString : EvalError → String
+| .OutOfBounds_Int64 n => s!"{n} is out of Int64 bounds, should be satisfied that -2{Nat.toSuperscriptString 63} ≤ n < 2{Nat.toSuperscriptString 63}"
+
+instance : ToString EvalError where
+  toString := EvalError.toString
