Tibi/Top.lean
@@ -11,7 +11,7 @@ partial def repl (stream : IO.FS.Stream) (n : Nat := 0) : IO UInt32 := do
   if not line.isEmpty then
     if let some r := parseLine line then
       match r with
-      | .ok (.ok expr, []) =>
+      | .ok (expr, []) =>
           match expr.typeCheck with
           | .found t _ =>
               match expr.eval with
@@ -19,9 +19,8 @@ partial def repl (stream : IO.FS.Stream) (n : Nat := 0) : IO UInt32 := do
               | .error e => IO.eprintln s!"Runtime Error: {e}"
           | .unknown =>
               IO.eprintln "Type Error"
-      | .ok (.error e, []) => IO.eprintln s!"Error: {e}"
-      | .ok (_,        cs) => IO.eprintln s!"Syntax Error: Unexpected tokens: {String.mk cs}"
-      | .error e           => IO.eprintln e.toString
+      | .ok (_, cs) => IO.eprintln s!"Syntax Error: Unexpected tokens: {String.mk cs}"
+      | .error e    => IO.eprintln e.toString
     repl stream n.succ
   else
     return 0
@@ -31,16 +30,18 @@ def run (inStream : IO.FS.Stream) : IO ByteArray :=
   >>= (
     fun r =>
       match r with
-      | .none                       => return none
-      | .some <| .ok (.ok expr, []) => return some expr
-      | .some <| .ok (.error e, []) => .throw s!"Error: {e}"
-      | .some <| .ok (_,        cs) => .throw s!"Syntax Error: Unexpected tokens: {String.mk cs}"
-      | .some <| .error e           => .throw e.toString
+      | .none                   => return none
+      | .some <| .ok (expr, []) => return some expr
+      | .some <| .ok (_,    cs) => .throw s!"Syntax Error: Unexpected tokens: {String.mk cs}"
+      | .some <| .error e       => .throw e.toString
   )
   >>= (
-    pure ∘ fun (e : Option Expr) =>
+    fun (e : Option Expr) =>
       match e with
-      | .none   => Wasm.empty
-      | .some e => Wasm.simple e.compile
+      | .none   => pure Wasm.empty
+      | .some e =>
+          match e.compile with
+          | .ok b    => return Wasm.simple b
+          | .error e => .throw s!"Compile Error: {e}"
   )
   >>= pure ∘ Wasm.build
